src/3d/Options.fst
@@ -16,6 +16,7 @@ let batch : ref bool = alloc false
 let clang_format : ref bool = alloc false
 let clang_format_executable : ref string = alloc ""
 let cleanup : ref bool = alloc false
+let skip_makefiles : ref bool = alloc false
 let arg0 : ref string = alloc "3d"
 
 (* We would like to parse --help as an option, but this would
@@ -37,6 +38,8 @@ let options0 =
    (noshort, "clang_format_executable", OneArg ((fun cmd -> batch := true; clang_format := true; clang_format_executable := cmd), "clang-format full path"), "Provide path to clang-format if not reachable through PATH");
    (noshort, "cleanup", ZeroArgs (fun _ -> cleanup := true), "Remove *.fst*, *.krml and kremlin-args.rsp (--batch only)");
    (noshort, "no_cleanup", ZeroArgs (fun _ -> cleanup := false), "Do not remove *.fst*, *.krml or kremlin-args.rsp");
+   (noshort, "skip_makefiles", ZeroArgs (fun _ -> skip_makefiles := true), "Do not generate Makefile.basic, Makefile.include");
+   (noshort, "no_skip_makefiles", ZeroArgs (fun _ -> skip_makefiles := false), "Generate Makefile.basic, Makefile.include (--batch only)");
    (noshort, "version", ZeroArgs (fun _ -> FStar.IO.print_string (Printf.sprintf "EverParse/3d %s\nCopyright 2018, 2019, 2020 Microsoft Corporation\n" Version.everparse_version); exit 0), "Show this version of EverParse");
    ]
 
@@ -64,7 +67,11 @@ let display_usage () : ML unit =
     end;
     if !cleanup then begin
       FStar.IO.print_string "--cleanup is currently toggled.\n"
-    end
+    end;
+    if !skip_makefiles then begin
+      FStar.IO.print_string "--skip_makefiles is currently toggled.\n"
+    end;
+    ()
   end
 
 let _ =
@@ -136,3 +143,6 @@ let get_clang_format_executable () =
 
 let get_cleanup () =
   !cleanup
+
+let get_skip_makefiles () =
+  !skip_makefiles
